proof/correctness/KyberINDCPA.ec
@@ -88,17 +88,413 @@ seq 1 10 : (#pre /\ rho{1} = publicseed{2} /\ sig{1} = noiseseed{2}).
 + by inline *; conseq => />; sim; auto => />; smt(W64.to_uintK W64.to_uint_small).
 swap {1} [7..8] -5.
 swap {2} [12..13] -8.
-seq 3 5 : (#pre /\ a{1} = lift_matrix (a0{2},a1{2},a2{2})). (* add bounds *)
+seq 3 5 : (#pre /\ a{1} = lift_matrix (a0{2},a1{2},a2{2}) /\
+            signed_bound768_cxq a0{2} 0 768 2 /\
+            signed_bound768_cxq a1{2} 0 768 2 /\
+            signed_bound768_cxq a2{2} 0 768 2). 
 inline M.gen_matrix. (* Need to define XOF such that this works. *)
 admit. (* To Do: HUGE *)
 swap {1} [5..10]  -2.
 swap {2} 6 -4.
 swap {2} [4..6] -1.
 swap {2} [9..22] -3.
-seq 8 19 : (#pre /\ s{1} = lift_vector skpv{2} /\ e{1} = lift_vector e{2}). (* add bounds *)
+seq 8 19 : (#pre /\ s{1} = lift_vector skpv{2} /\ e{1} = lift_vector e{2} /\
+                signed_bound768_cxq skpv{2} 0 768 2 /\
+                signed_bound768_cxq e{2} 0 768 2).
 admit. (* To Do: Define PRF so that this works *)
-seq 5 14 : #pre. (* To Do: specify algebraic part *)
-admit. (*  already done. Recover it *)
+seq 5 14 : (#pre /\ t{1} = lift_vector pkpv{2} /\
+                signed_bound768_cxq pkpv{2} 0 768 2). 
+seq 2 1: #pre; first by auto.
+sp 0 2.
+seq 1 1 : #pre.
+exists* (lift_array768 skpv{2}).
+elim* => s2.
+call {2} (_: lift_array768 r = s2 /\
+              signed_bound768_cxq r 0 768 2 ==>
+             lift_array768 res = s2 /\
+              signed_bound768_cxq res 0 768 2  ).
+apply (polyvec_ntt_correct s2).
+conseq => />.
+
+(*
+seq 3 : #pre; first by auto => />.
+(******)
+seq 2 : (#pre /\
+   lift_vector a0 = row_i (ntt_matrix (H sd)) 0 /\
+   lift_vector a1 = row_i (ntt_matrix (H sd)) 1 /\
+   lift_vector a2 = row_i (ntt_matrix (H sd)) 2 /\
+   signed_bound768_cxq a0 0 768 2 /\
+   signed_bound768_cxq a1 0 768 2 /\
+   signed_bound768_cxq a2 0 768 2).
+ecall (gen_matrix sd).
+auto => /> &hr ??? -> *.
+rewrite /row_i /lift_vector /lift_matrix /ntt_matrix /lift_polyvec => />.
+do split.
+rewrite eq_vectorP // => *.
+rewrite !offunvE => />.
+by rewrite !offunmE => />.
+rewrite eq_vectorP // => *.
+rewrite !offunvE => />.
+by rewrite !offunmE => />.
+rewrite eq_vectorP // => *.
+rewrite !offunvE => />.
+by rewrite !offunmE => />.
+(******)
+seq 1 : (#{/~skpv}pre /\
+   lift_vector skpv = polyvec_ntt s_ /\
+   signed_bound768_cxq skpv 0 768 2
+   ).
+ecall(polyvec_ntt_correct (lift_array768 skpv)).
+skip => /> &hr ?.
+rewrite /row_i /lift_vector /lift_polyvec /polyvec_ntt /pos_bound768_cxq  /signed_bound768_cxq /lift_array768 /sub => /> *.
+split; last  by smt(@Array768). 
+rewrite eq_vectorP  => /> *.
+rewrite !offunvE => />.
+rewrite offunvK /vclamp H13 =>  />.
+case (i = 0).
+move => -> />.
+rewrite -H9 => />.
+congr. 
+apply Array256.ext_eq => x xb.
+rewrite !initiE => />. 
+rewrite nth_mkseq => />.
+rewrite  mapiE; first by smt().
+by auto => />.
+move => *.
+case (i = 1).
+move => -> />.
+rewrite -H10 => />.
+congr. 
+apply Array256.ext_eq => x xb.
+rewrite !initiE => />. 
+rewrite nth_mkseq => />. 
+rewrite  mapiE; first by smt().
+by auto => />.
+case (i = 2).
+move => -> />.
+rewrite -H11 => />.
+congr. 
+apply Array256.ext_eq => x xb.
+rewrite !initiE => />. 
+rewrite nth_mkseq => />. 
+rewrite  mapiE; first by smt().
+by auto => />.
+smt().
+(******)
+seq 1 : (#{/~e}pre /\
+   lift_vector e = polyvec_ntt e_ /\
+   signed_bound768_cxq e 0 768 2
+   ).
+ecall(polyvec_ntt_correct (lift_array768 e)).
+skip => /> &hr ?.
+rewrite /row_i /lift_vector /lift_polyvec /polyvec_ntt /pos_bound768_cxq  /signed_bound768_cxq /lift_array768 /sub => /> *.
+split;  last  by smt(@Array768). 
+rewrite eq_vectorP  =>  *.
+rewrite !offunvE => />.
+rewrite offunvK /vclamp H14 =>  />.
+case (i = 0).
+move => -> />.
+rewrite -H10 => />.
+congr. 
+apply Array256.ext_eq => x xb.
+rewrite !initiE => />. 
+rewrite nth_mkseq => />.
+rewrite  mapiE; first by smt().
+by auto => />.
+move => *.
+case (i = 1).
+move => -> />.
+rewrite -H11 => />.
+congr. 
+apply Array256.ext_eq => x xb.
+rewrite !initiE => />. 
+rewrite nth_mkseq => />. 
+rewrite  mapiE; first by smt().
+by auto => />.
+case (i = 2).
+move => -> />.
+rewrite -H12 => />.
+congr. 
+apply Array256.ext_eq => x xb.
+rewrite !initiE => />. 
+rewrite nth_mkseq => />. 
+rewrite  mapiE; first by smt().
+by auto => />.
+smt().
+(*****)
+seq 1 : (#pre /\
+    signed_bound_cxq poly0 0 256 2 /\ lift_array256 poly0 = ntt ((row_i (H sd) 0) `<*>` s_)).
+call (innerprod_corr (row_i (H sd) 0) s_ H).
+auto => /> &hr.
+rewrite  /lift_polyvec /polyvec_ntt /pos_bound768_cxq  /signed_bound768_cxq /lift_array768 /sub => /> *.
+split. 
+(*****)
+rewrite eq_vectorP  =>  *.
+rewrite !offunvE => />.
+rewrite offunvK /vclamp H10.
+case (i = 0).
+move => iis0.
+apply Array256.ext_eq => x xb.
+move : H0.
+rewrite iis0 /row_i => /> *.
+rewrite !initiE => />. 
+rewrite (_: (ntt ((H sd))%MLWEPKE.H_MLWE.[0, 0]) = 
+   (offunv (fun (i0 : int) => (ntt_matrix ((H sd))%MLWEPKE.H_MLWE).[0, i0])).[0]).
+by rewrite /ntt_matrix offunvE //= offunmE  => />.
+rewrite -H0.
+rewrite offunvE => />.
+by rewrite initiE.
+move => *.
+case (i = 1).
+move => iis1.
+apply Array256.ext_eq => x xb.
+move : H0.
+rewrite iis1 /row_i => /> *.
+rewrite !initiE => />. 
+rewrite (_: (ntt ((H sd))%MLWEPKE.H_MLWE.[0, 1]) = 
+   (offunv (fun (i0 : int) => (ntt_matrix ((H sd))%MLWEPKE.H_MLWE).[0, i0])).[1]).
+rewrite /ntt_matrix offunvE //= offunmE  => />.
+rewrite -H0.
+rewrite offunvE => />.
+by rewrite initiE.
+move => *.
+case (i = 2).
+move => iis2.
+apply Array256.ext_eq => x xb.
+move : H0.
+rewrite iis2 /row_i => /> *.
+rewrite !initiE => />. 
+rewrite (_: (ntt ((H sd))%MLWEPKE.H_MLWE.[0, 2]) = 
+   (offunv (fun (i0 : int) => (ntt_matrix ((H sd))%MLWEPKE.H_MLWE).[0, i0])).[2]).
+rewrite /ntt_matrix offunvE //= offunmE  => />.
+rewrite -H0.
+rewrite offunvE => />.
+by rewrite initiE.
+smt().
+(*****)
+by rewrite H6.
+(****)
+(*****)
+seq 1 : (#pre /\
+    signed_bound_cxq poly1 0 256 2 /\ lift_array256 poly1 = ntt ((row_i (H sd) 1) `<*>` s_)).
+call (innerprod_corr (row_i (H sd) 1) s_ H).
+auto => /> &hr.
+rewrite  /lift_polyvec /polyvec_ntt /pos_bound768_cxq  /signed_bound768_cxq /lift_array768 /sub => /> *.
+split. 
+(*****)
+rewrite eq_vectorP  =>  *.
+rewrite !offunvE => />.
+rewrite offunvK /vclamp H12.
+case (i = 0).
+move => iis0.
+apply Array256.ext_eq => x xb.
+move : H1.
+rewrite iis0 /row_i => /> *.
+rewrite !initiE => />. 
+rewrite (_: (ntt ((H sd))%MLWEPKE.H_MLWE.[1, 0]) = 
+   (offunv (fun (i0 : int) => (ntt_matrix ((H sd))%MLWEPKE.H_MLWE).[1, i0])).[0]).
+by rewrite /ntt_matrix offunvE //= offunmE  => />.
+rewrite -H1.
+rewrite offunvE => />.
+by rewrite initiE.
+move => *.
+case (i = 1).
+move => iis1.
+apply Array256.ext_eq => x xb.
+move : H1.
+rewrite iis1 /row_i => /> *.
+rewrite !initiE => />. 
+rewrite (_: (ntt ((H sd))%MLWEPKE.H_MLWE.[1, 1]) = 
+   (offunv (fun (i0 : int) => (ntt_matrix ((H sd))%MLWEPKE.H_MLWE).[1, i0])).[1]).
+rewrite /ntt_matrix offunvE //= offunmE  => />.
+rewrite -H1.
+rewrite offunvE => />.
+by rewrite initiE.
+move => *.
+case (i = 2).
+move => iis2.
+apply Array256.ext_eq => x xb.
+move : H1.
+rewrite iis2 /row_i => /> *.
+rewrite !initiE => />. 
+rewrite (_: (ntt ((H sd))%MLWEPKE.H_MLWE.[1, 2]) = 
+   (offunv (fun (i0 : int) => (ntt_matrix ((H sd))%MLWEPKE.H_MLWE).[1, i0])).[2]).
+rewrite /ntt_matrix offunvE //= offunmE  => />.
+rewrite -H1.
+rewrite offunvE => />.
+by rewrite initiE.
+smt().
+(*****)
+by rewrite H6.
+(****)
+(*****)
+seq 1 : (#pre /\
+    signed_bound_cxq poly2 0 256 2 /\ lift_array256 poly2 = ntt ((row_i (H sd) 2) `<*>` s_)).
+call (innerprod_corr (row_i (H sd) 2) s_ H).
+auto => /> &hr.
+rewrite  /lift_polyvec /polyvec_ntt /pos_bound768_cxq  /signed_bound768_cxq /lift_array768 /sub => /> *.
+split. 
+(*****)
+rewrite eq_vectorP  =>  *.
+rewrite !offunvE => />.
+rewrite offunvK /vclamp H14.
+case (i = 0).
+move => iis0.
+apply Array256.ext_eq => x xb.
+move : H2.
+rewrite iis0 /row_i => /> *.
+rewrite !initiE => />. 
+rewrite (_: (ntt ((H sd))%MLWEPKE.H_MLWE.[2, 0]) = 
+   (offunv (fun (i0 : int) => (ntt_matrix ((H sd))%MLWEPKE.H_MLWE).[2, i0])).[0]).
+by rewrite /ntt_matrix offunvE //= offunmE  => />.
+rewrite -H2.
+rewrite offunvE => />.
+by rewrite initiE.
+move => *.
+case (i = 1).
+move => iis1.
+apply Array256.ext_eq => x xb.
+move : H2.
+rewrite iis1 /row_i => /> *.
+rewrite !initiE => />. 
+rewrite (_: (ntt ((H sd))%MLWEPKE.H_MLWE.[2, 1]) = 
+   (offunv (fun (i0 : int) => (ntt_matrix ((H sd))%MLWEPKE.H_MLWE).[2, i0])).[1]).
+rewrite /ntt_matrix offunvE //= offunmE  => />.
+rewrite -H2.
+rewrite offunvE => />.
+by rewrite initiE.
+move => *.
+case (i = 2).
+move => iis2.
+apply Array256.ext_eq => x xb.
+move : H2.
+rewrite iis2 /row_i => /> *.
+rewrite !initiE => />. 
+rewrite (_: (ntt ((H sd))%MLWEPKE.H_MLWE.[2, 2]) = 
+   (offunv (fun (i0 : int) => (ntt_matrix ((H sd))%MLWEPKE.H_MLWE).[2, i0])).[2]).
+rewrite /ntt_matrix offunvE //= offunmE  => />.
+rewrite -H2.
+rewrite offunvE => />.
+by rewrite initiE.
+smt().
+(*****)
+by rewrite H6.
+(*********************************)
+seq 1 : (#pre /\
+             signed_bound768_cxq pkpv 0 768 2 /\
+             polyvec_ntt (H(sd) *^ s_) = lift_vector pkpv).
+ecall (polyvec_frompolys_corr_h poly0 poly1 poly2
+         (ntt (row_i ((H sd))%MLWEPKE.H_MLWE 0 `<*>` s_))
+         (ntt (row_i ((H sd))%MLWEPKE.H_MLWE 1 `<*>` s_))
+         (ntt (row_i ((H sd))%MLWEPKE.H_MLWE 2 `<*>` s_)) 2  ).
+auto => /> &hr.
+move => *.
+split; first by smt().
+rewrite /(`<*>`); move => *.
+
+rewrite /lift_vector /polyvec_ntt /lift_polyvec => />.
+rewrite eq_vectorP  =>  *.
+rewrite !offunvE => />.
+case (i = 0).
+move => -> />. 
+apply Array256.ext_eq => k kb.
+rewrite initiE => />.
+rewrite (H23 k kb).
+rewrite /row_i => />.
+do congr.
+rewrite  /( *^) offunvK /vclamp. 
+rewrite /dotp /= !Big.BAdd.big_consT /= !Big.BAdd.big_nil /=. 
+by rewrite !offunvE => />.
+case (i = 1).
+move => -> />. 
+apply Array256.ext_eq => k kb.
+rewrite initiE => />.
+rewrite  (_: 256 + k = k + 256); first by smt().
+rewrite (H24 k kb) =>/> *.
+rewrite /row_i => />.
+do congr.
+rewrite  /( *^) offunvK /vclamp. 
+rewrite /dotp /= !Big.BAdd.big_consT /= !Big.BAdd.big_nil /=. 
+by rewrite !offunvE => />.
+case (i = 2).
+move => -> />. 
+apply Array256.ext_eq => k kb.
+rewrite initiE => />.
+rewrite  (_: 512 + k = k + 512); first by smt().
+rewrite (H25 k kb) =>/> *.
+rewrite /row_i => />.
+do congr.
+rewrite  /( *^) offunvK /vclamp. 
+rewrite /dotp /= !Big.BAdd.big_consT /= !Big.BAdd.big_nil /=. 
+by rewrite !offunvE => />.
+smt().
+seq 1 : (#{/~pkpv}pre /\
+    signed_bound768_cxq pkpv 0 768 4 /\ polyvec_ntt ((H sd)%MLWEPKE.H_MLWE *^ s_ + e_) = lift_vector pkpv).
+exists *(lift_array768 pkpv) ,(lift_array768 e). elim * => _p _e.
+call (polyvec_add_corr _p _e 2 2).
+auto => /> *.
+(***************************************)
+rewrite polyvec_ntt_add.
+rewrite H17 -H8 /lift_vector /polyvec_ntt /lift_polyvec //=.
+rewrite !eq_vectorP  //=  => *.
+rewrite !offunvE //=.
+rewrite /(Poly.(+)) map2E //=.
+apply Array256.ext_eq => x xb. 
+rewrite !initiE //=.
+case (i = 0).
+move => -> //=.
+rewrite !initiE => //=.
+move : (H19 x _); first by smt().
+rewrite /lift_array768 //= !mapiE //=; first  2 by smt().
+rewrite  -ZModField.inzmodD.
+by move => ->.
+case (i = 1).
+move => -> //=.
+rewrite !initiE => //=.
+move : (H19 (256 + x) _); first by smt().
+rewrite /lift_array768 //= !mapiE //=; first  2 by smt().
+rewrite  -ZModField.inzmodD.
+by move => ->.
+case (i = 2).
+move => -> //=.
+rewrite !initiE => //=.
+move : (H19 (512 + x) _); first by smt().
+rewrite /lift_array768 //= !mapiE //=; first  2 by smt().
+rewrite  -ZModField.inzmodD.
+by move => ->.
+by smt().
+(***************************************)
+ecall (polyvec_reduce_corr (lift_array768 pkpv)).
+auto => /> *.
+split; last by rewrite /signed_bound768_cxq;smt(@Array768).
+move : H17 H18; rewrite /polyvec_ntt  /lift_vector /lift_array768 /lift_polyvec  !mapE.
+rewrite (Array768.tP 
+  ((Array768.init (fun (i : int) => (fun (x : W16.t) => (ZModField.inzmod (to_sint x))%ZModField) pkpv{hr}.[i])))
+  ((Array768.init (fun (i : int) => (fun (x : W16.t) => (ZModField.inzmod (to_sint x))%ZModField) result.[i])))).
+rewrite !eq_vectorP  //=  => *.
+rewrite (H17 i H20) //.
+rewrite !offunvE //=.
+apply Array256.ext_eq => k kb.
+case  (i = 0).
+move => -> //=.
+move  : (H18 k _) => //; first by smt().
+rewrite !initiE; first 4 by smt().
+by move => ->.
+move => *.
+case  (i = 1).
+move => -> //=.
+move  : (H18 (256 + k) _) => //; first by smt().
+rewrite !initiE; first 4 by smt().
+by move => ->.
+move => *.
+case  (i = 2).
+move => -> //=.
+move  : (H18 (512 + k) _) => //; first by smt().
+rewrite !initiE; first 4 by smt().
+by move => ->.
+by smt().
+qed.
+*)
 admit. (* just storing in memory *)
 qed.
 
